## Standing assumptions

## 1A

### Exercise 1A, 1

$ \alpha = a_r + a_i \ i \ \text{ where } \ a_r, a_i \in \R $

$ \beta = b_r + b_i \ i \ \text{ where } \ b_r, b_i \in \R $

$ \alpha + \beta = \beta + \alpha $

---

$ \alpha + \beta = (a_r + b_r) + (a_i + b_i) \ i $

$ = (b_r + a_r) + (b_i + a_i) \ i $

$ = \beta + \alpha $


### Exercise 1A, 2

$ \alpha = a_r + a_i \ i  \text{ where } \ a_r, a_i \in \R $

$ \beta = b_r + b_i \ i \ \text{ where } \ b_r, b_i \in \R $

$ \lambda = l_r + l_i \ i \ , l_r \in \R \ , l_i \in \R $

$ (\alpha + \beta) + \lambda = \alpha + (\beta + \lambda) $

---

$ (\alpha + \beta) + \lambda = ((a_r + b_r) + (a_i + b_i) \ i) + (l_r + l_i \ i) $

$ = ((a_r + b_r) + l_r) + ((a_i + b_i) + l_i) \ i $

$ = (a_r + (b_r + l_r)) + (a_i + (b_i + l_i)) \ i $

$ = \alpha + (\beta + \lambda) $


### Exercise 1A, 3

$ \alpha = a_r + a_i \ i  \text{ where } \ a_r, a_i \in \R $

$ \beta = b_r + b_i \ i \ \text{ where } \ b_r, b_i \in \R $

$ \lambda = l_r + l_i \ i \ , l_r \in \R \ , l_i \in \R $

$ (\alpha \beta) \lambda = \alpha (\beta \lambda) $

---

$ (\alpha \beta) \lambda = ((a_r + a_i \ i)(b_r + b_i \ i))(l_r + l_i \ i) $


$ = ((a_r b_r - a_i b_i) + (a_r b_i + a_i b_r) \ i)(l_r + l_i \ i) $

$ = ((a_r b_r - a_i b_i) l_r - (a_r b_i + a_i b_r) l_i) + ((a_r b_r - a_i b_i) l_i + (a_r b_i + a_i b_r) l_r) \ i $

$ = (a_r b_r l_r - a_i b_i l_r - a_r b_i l_i - a_i b_r l_i) + (a_r b_r l_i - a_i b_i l_i + a_r b_i l_r + a_i b_r l_r) \ i $

$ = (a_r(b_r l_r - b_i l_i) - a_i(b_r l_i + b_i l_r)) + (a_r(b_r l_i + b_i l_r) + a_i(b_r l_r - b_i l_i)) \ i $

$ = (a_r + a_i \ i)((b_r l_r - b_i l_i) + (b_r l_i + b_i l_r) \ i) $

$ = (a_r + a_i \ i)((b_r + b_i \ i)(l_r + l_i \ i)) $

$ = \alpha (\beta \lambda) $

### Exercise 1A, 4

$ \alpha = a_r + a_i \ i  \text{ where } \ a_r, a_i \in \R $

$ \beta = b_r + b_i \ i \ \text{ where } \ b_r, b_i \in \R $

$ \lambda = l_r + l_i \ i \ , l_r \in \R \ , l_i \in \R $

$ \lambda  (\alpha + \beta) = \lambda \alpha + \lambda \beta $

---

$ \lambda  (\alpha + \beta) = (l_r + l_i \ i)((a_r + b_r) + (a_i + b_i) \ i) $

$ = (l_r(a_r + b_r) - l_i(a_i + b_i)) + (l_r(a_i + b_i) + l_i(a_r + b_r)) \ i $

$ = (l_r a_r - l_i a_i + l_r b_r - l_i b_i) + (l_r a_i + l_i a_r + l_r b_i + l_i b_r) \ i $

$ = (l_r a_r - l_i a_i) + (l_r b_r - l_i b_i) + (l_r a_i + l_i a_r) \ i + (l_r b_i + l_i b_r) \ i $

$ = ((l_r a_r - l_i a_i) + (l_r a_i + l_i a_r) \ i) + ((l_r b_r - l_i b_i) + (l_r b_i + l_i b_r) \ i) $

$ = \lambda \alpha + \lambda \beta $

### Exercise 1A, 5

$ \alpha = a_r + a_i \ i $

$ \beta = b_r + b_i \ i $

$ \alpha + \beta = 0 $

---

$ \alpha + \beta = (a_r + b_r) + (a_i + b_i) \ i = 0 $

$ \Rightarrow a_r + b_r = 0 \ \text{ and } \ a_i + b_i = 0 $

$ \Rightarrow b_r = -a_r \ \text{and} \ b_i = -a_i $

$ \Rightarrow \beta = -\alpha $

Is unique

### Exercise 1A, 6

Also Multiplicative inverse on page 3

$ \alpha = a_r + a_i \ i $

$ \beta = b_r + b_i \ i $

$ \alpha \ \beta = 1 $

---

$ a_r b_r - a_i b_i + (a_r b_i + a_i b_r) \ i = 1 + 0 \ i $

$ \Rightarrow a_r b_r - a_i b_i = 1 $

$ \Rightarrow a_r b_i + a_i b_r = 0 $

$ \Rightarrow  a_r^2 b_r - a_r a_i b_i + a_i a_r b_i + a_i^2 b_r = a_r$

$ \Rightarrow b_r = \frac{a_r}{a_r^2 + a_i^2} $

$ \Rightarrow b_i = -\frac{a_i}{a_r^2 + a_i^2} $

### Exercise 1A, 7

$ \alpha = \frac{-1 + \sqrt{3} \ i}{2}$

----

$ \alpha^2 = \left( \frac{-1 + \sqrt{3} \ i}{2} \right) \left( \frac{-1 + \sqrt{3} \ i}{2} \right) $

$ = \frac{1 - 2 \sqrt{3} \ i + 3 i^2}{4} $

$ = \frac{-1 - \sqrt{3} \ i}{2} $

$ \alpha^3 = \left( \frac{-1 - \sqrt{3} \ i}{2} \right) \left( \frac{-1 + \sqrt{3} \ i}{2} \right) $

$ = \frac{(-1 - \sqrt{3} \ i)(-1 + \sqrt{3} \ i)}{4} $

$ = \frac{1 - (\sqrt{3} \ i)^2}{4} $

$ = \frac{1 - 3 i^2}{4} $

$ = 1 $

### Exercise 1A, 7

Square roots of $ i $

---

$ x^2 = i $

$ x = a + bi $

$ (a + bi)^2 = i $

$ a^2 + 2abi + (bi)^2 = i $

$ a^2 + 2abi - b^2 = i $


### Exercise 1A, 8

Solve

$ (4, -3, 1, 7) + 2x = (5, 9, -6, 8) $

---

$ ((-4, 3, -1, -7) + (4, -3, 1, 7)) + 2x = (-4, 3, -1, -7) + (5, 9 -6, 8) $

$ 0 + 2x = (1, 12, -7, 1) $

$ \frac{1}{2} \ 2 x = \frac{1}{2} \ (1, 12, -7, 1) $

$ x = ( \frac{1}{2}, 6, -\frac{7}{2}, \frac{1}{2} ) $

### Exercise 1A, 9
